Reorganized files. Input abstract stack in SFS.

sfs.v
@@ -1,4 +1,10 @@
-From Coq_EVM Require Import evmModel.
+(* Enrique Martin - Univ. Complutense de Madrid
+   Licensed under the GNU GENERAL PUBLIC LICENSE 3.0.
+
+   You may obtain a copy of the License at
+   https://www.gnu.org/licenses/gpl-3.0.txt
+*)
+
 Require Import Coq.Lists.List.
 Require Import bbv.Word.
 Require Import Coq.Init.Nat. (* for <? *)
@@ -7,355 +13,12 @@ Require Export Coq.Strings.Ascii.
 Require Export Coq.Strings.String.
 Open Scope string_scope.
 
-(* POSSIBLE IMPROVEMENTS:
-   - Use faster mappings. Instead of list (key, value) use AVL or RB trees as in evmModel (FMapAVL)
-   - Define domains as sets of strings
-*)
 
-
-(******************
-  LISTS OF STRINGS 
- ******************)
-(* 'In' function for list of strings but returning a boolean *)
-Fixpoint In_list_str_eval (e: string) (l: list string) : bool :=
-match l with 
-  | nil => false
-  | v::tail => orb (v =? e) (In_list_str_eval e tail)
-end.
-
-(* In and In_list_str_eval are equivalent *)
-Lemma in_str_equiv_true: forall (e: string) (l: list string),
-  In e l <-> In_list_str_eval e l = true.
-Proof.
-intros e l. split. 
- + induction l as [ | h t IH].
-   - intros H. apply in_nil in H. contradiction.
-   - intros H. destruct (eqb e h) eqn: elem_eq.
-     * unfold In_list_str_eval. rewrite eqb_sym in elem_eq. rewrite elem_eq. reflexivity.
-     * simpl. rewrite eqb_sym in elem_eq. rewrite elem_eq. simpl.
-       simpl in H. destruct H.
-       ++ rewrite <- eqb_eq in H. rewrite H in elem_eq.
-          discriminate elem_eq.
-       ++ apply IH in H. assumption.
- + induction l as [ | h t IH].
-   - simpl. intros H. discriminate.
-   - unfold In_list_str_eval. destruct (h =? e) eqn:eq_eh.
-     * simpl. intros Htrue. rewrite eqb_sym in eq_eh. apply eqb_eq in eq_eh.
-       left. symmetry. assumption.
-     * simpl. fold In_list_str_eval. intros Hin. apply IH in Hin. right. assumption.
-Qed.
+Require Import Coq_EVM.lib.evmModel.
+Require Import Coq_EVM.string_map.
 
 
 
-(* In and In_list_str_eval are equivalent also in the negative case *)
-Lemma in_str_equiv_false: forall (e: string) (l: list string),
-  ~In e l <-> In_list_str_eval e l = false.
-Proof.
-intros e l. split. 
-+ (* -> *)
-  induction l as [ | h t IH].
-  - intros Henotinnil. reflexivity.
-  - intros Henotin. destruct (eqb e h) eqn: elem_eq.
-    * simpl in Henotin.
-      pose proof (Decidable.not_or (h = e) (In e t) Henotin) as Henotin_despl.
-      destruct Henotin_despl as [Hehdiff Henotint].
-      rewrite <- eqb_eq in Henotin.
-      rewrite <- eqb_neq in Hehdiff.
-      rewrite -> eqb_sym in elem_eq.
-      rewrite elem_eq in Hehdiff.
-      discriminate.
-    * simpl in Henotin. simpl.
-      pose proof (Decidable.not_or (h = e) (In e t) Henotin) as Henotin_despl.
-      destruct Henotin_despl as [Hehdiff Henotint].
-      rewrite -> eqb_sym in elem_eq.
-      rewrite -> elem_eq. simpl.
-      apply IH in Henotint as Hfinal.
-      assumption.
-+ (* <- *) induction l as [ | h t IH].
-  - intro Hinevalfalse. simpl. unfold not. trivial.
-  - intro Hinevalfalse. simpl in Hinevalfalse.
-    destruct (eqb e h) eqn: elem_eq.
-    * rewrite -> eqb_sym in elem_eq.
-      rewrite -> elem_eq in Hinevalfalse. simpl in Hinevalfalse.
-      discriminate.
-    * rewrite -> eqb_sym in elem_eq.
-      rewrite -> elem_eq in Hinevalfalse. simpl in Hinevalfalse.
-      apply IH in Hinevalfalse.
-      simpl.
-      unfold not.
-      intro Hin.
-      destruct Hin as [Heq|HInet].
-      ++ rewrite -> Heq in elem_eq.
-         rewrite -> eqb_refl in elem_eq.
-         discriminate.
-      ++ contradiction.
-Qed.
-
-(* In is decidable: In e l /\ ~ In e l
-   Useful to apply some lemma from library Coq.Logic.Decidable *)
-Lemma in_decidable: forall (e: string) (l: list string),
-Decidable.decidable (In e l).
-Proof.
-intros e l.
-unfold Decidable.decidable.
-rewrite in_str_equiv_true.
-destruct (In_list_str_eval e l) eqn: eqevalin.
-- left. reflexivity.
-- right. apply Bool.diff_false_true.
-Qed.
-
-
-(* In_list_string_eval is dedicable
-   Useful to apply some lemma from library Coq.Logic.Decidable *)
-Lemma in_list_str_eval_decidable: forall (e: string) (l: list string) (b:bool),
-Decidable.decidable (In_list_str_eval e l = b).
-Proof.
-intros e l b.
-unfold Decidable.decidable.
-destruct (In_list_str_eval e l) eqn: eqevalin.
-- destruct b eqn: eqb. 
-  + left. reflexivity.
-  + right. apply Bool.diff_true_false.
-- destruct b eqn: eqb. 
-  + right. apply Bool.diff_false_true.
-  + left. reflexivity.
-Qed.
-
-
-(* No element h of l1 appears in l2 *)
-Fixpoint not_in_list (l1 l2: list string) : Prop :=
-match l1 with
-  | nil => True
-  | h::t => ~ (In h l2) /\ (not_in_list t l2)
-end.
-
-Definition disjoint_eval (l1 l2: list string) : Prop :=
-(not_in_list l1 l2).
-
-Definition disjoint (l1 l2: list string) : Prop :=
-forall (x: string), In x l1 -> ~ In x l2.
-
-Lemma disjoint_extend: forall (l1 l2: list string) (elem: string),
-disjoint l1 l2 ->
-~ In elem l2 ->
-disjoint (elem::l1) l2.
-Proof.
-intros l1 l2 elem Hdisjoint Hnotin.
-unfold disjoint.
-intro e. simpl.
-rewrite <- eqb_eq.
-destruct (elem =? e) eqn: eqeleme.
-- simpl. rewrite -> eqb_eq in eqeleme.
-  rewrite <- eqeleme. intro Htrue. assumption.
-- unfold orb. intro He.
-  destruct He as [Hfalse | Heinl1].
-  + discriminate.
-  + unfold disjoint in Hdisjoint.
-    pose proof (Hdisjoint e) as Henotin.
-    apply Henotin in Heinl1.
-    assumption.
-Qed.
-
-Search In.
-
-
-Lemma disjoint_split: forall (l1 l2: list string) (elem: string),
-disjoint (elem::l1) l2 ->
-~ In elem l2 /\ disjoint l1 l2.
-Proof.
-intros l1 l2 elem.
-unfold disjoint.
-intros Himpl.
-split.
-- pose proof (Himpl elem).
-  pose proof (in_eq elem l1) as Helemincons.
-  apply H in Helemincons.
-  assumption.
-- intros y.
-  pose proof (Himpl y) as Himply.
-  intros Hyinl1.
-  pose proof (in_cons elem y l1) as Hyineleml1.
-  apply Hyineleml1 in Hyinl1.
-  apply Himply in Hyinl1.
-  assumption.
-Qed.
-
-
-
-Lemma disjoint_equiv: forall (l1 l2: list string),
-disjoint_eval l1 l2 <-> disjoint l1 l2.
-Proof.
-split.
-- (* -> *) 
-  induction l1 as [|h t IH].
-  + simpl. intro Htrue. unfold disjoint.
-    intro elem. simpl. intro Hfalse. contradiction.
-  + simpl. intros [Hnotinl2 Hdisjoint].
-    apply IH in Hdisjoint.
-    apply disjoint_extend; try assumption.
-- (* <- *)
-  induction l1 as [|h t IH].
-  + simpl. trivial. 
-  + simpl. intro Hdisjoint.
-    pose proof (disjoint_split t l2 h) as Hsplitdisjoint.
-    apply Hsplitdisjoint in Hdisjoint.
-    destruct Hdisjoint as [Hnotinl2 Hdisjointl2].
-    apply IH in Hdisjointl2.
-    split; try assumption.
-Qed.
-
-
-
-Lemma disjoint_sym: forall (l1 l2: list string),
-  (disjoint l1 l2) -> (disjoint l2 l1).
-Proof.
-intros l1 l2.
-unfold disjoint.
-intro Hdisjoint.
-intros elem Hxinl2.
-destruct (In_list_str_eval elem l1) eqn: Helem_in_l1.
-- rewrite <- in_str_equiv_true in Helem_in_l1.
-  pose proof (Hdisjoint elem Helem_in_l1). contradiction.
-- rewrite <- in_str_equiv_false in Helem_in_l1.
-  assumption.
-Qed.
-
-
-Lemma disjoint_then_not_in: forall (l m: list string) (name: string),
-disjoint l m ->
-In name l ->
-~ In name m.
-Proof.
-intros l m name Hdisjoint.
-unfold disjoint in Hdisjoint.
-pose proof (Hdisjoint name).
-assumption.
-Qed.
-
-
-
-
-
-(**********
-  MAPPINGS 
- **********)
-
-(* Mapping as list of tuples with duplicates. Probably FMapAVL is better and faster, but we
-   need to define keys as OrderedType and I don't know how to do that *)
-Definition map (T : Type) : Type := list (string * T).
-Definition empty_map {A : Type} : map A := nil.
-Definition update {A : Type} (m : map A) (x : string) (v : A): map A :=
-  (x,v) :: m.
-Fixpoint lookup {A : Type} (m : map A) (x : string) : option A :=
-match m with
-  | nil => None
-  | (y,v)::tail => if x =? y then Some v else (lookup tail x)
-end.
-
-
-Fixpoint domain {A: Type} (m: map A) : list string :=
-match m with
-  | nil => nil
-  | (k,v)::tail => k::(domain tail)
-end.
-
-
-
-(* looking for a key after updating the map returns the inserted value *)
-Lemma update_lookup: forall (T: Type) (m:  map T) (key: string) (value: T),
-  lookup (update m key value) key = Some value.
-Proof.
-  intros T m key value.
-  unfold update. unfold lookup. destruct (key =? key) eqn: EqKey.
-  - reflexivity.
-  - rewrite -> (eqb_refl key) in EqKey. (* from Coq.Strings.String *)
-    discriminate.
-Qed.
-
-
-(* looking for a different key after updating the map is the same as looking in the
-   original map *)
-Lemma update_lookup_diff: forall (T: Type) (m:  map T) (key1 key2: string) (value: T),
-  key1 =? key2 = false -> lookup (update m key1 value) key2 = lookup m key2.
-Proof.
-  intros T m key1 key2 value HKey. unfold update. unfold lookup.
-  rewrite -> (eqb_sym key1 key2) in HKey. (* from Coq.Strings.String *)
-  rewrite HKey. reflexivity.
-Qed.
-
-
-Lemma lookup_then_key_in_domain: forall {A: Type} (m: map A) (key: string) 
-      (value: A),
-lookup m key = Some value -> In key (domain m).
-Proof.
-intros A m key value.
-induction m as [ | pair tail].
-- simpl. intro Hfalse. discriminate.
-- unfold lookup.
-  destruct (pair) as [k v].
-  destruct (key =? k) eqn: eqkey.
-    + apply eqb_eq in eqkey. rewrite -> eqkey. intro Hvalue.
-      unfold domain. unfold In. left. reflexivity.
-    + fold @lookup. (* The @ is needed because of the implicit parameter, otherwise
-                       it cannot infer the type A *)
-      intros Hlookuptail.
-      unfold domain.
-      unfold In.
-      right.
-      fold @domain. 
-      apply IHtail in Hlookuptail.
-      assumption.
-Qed.
-
-
-
-Lemma in_domain_then_lookup: forall {A: Type} (m: map A) (key: string),
-In key (domain m) -> exists (value:A), lookup m key = Some value.
-Proof.
-intros A m key.
-induction m as [ | pair tail].
-- simpl. intro Hfalse. contradiction.
-- destruct (pair) as [k v]. unfold domain.
-  destruct (key =? k) eqn: eqkey.
-  + apply eqb_eq in eqkey. rewrite -> eqkey. intro Hdespl. 
-    exists v. unfold lookup.
-    rewrite -> eqb_refl. reflexivity.
-  + fold @domain. intro Hdespl.
-    destruct Hdespl as [Hkeyfalse|Hintail].
-    * rewrite eqb_neq in eqkey. rewrite Hkeyfalse in eqkey. contradiction.
-    * unfold In in IHtail.
-      apply IHtail in Hintail.
-      unfold lookup.
-      rewrite -> eqkey.
-      fold @lookup.
-      assumption.
-Qed.
-
-
-
-Lemma not_in_domain_then_lookup_none: forall {A: Type} (m: map A) (key: string),
-~In key (domain m) -> lookup m key = None.
-Proof.
-intros A m key.
-induction m as [ | pair tail].
-- simpl. intro Hfalse. reflexivity.
-- destruct (pair) as [k v]. unfold domain.
-  destruct (key =? k) eqn: eqkey.
-  + rewrite -> in_str_equiv_true. 
-    unfold In_list_str_eval.
-    rewrite eqb_sym.
-    rewrite -> eqkey.
-    simpl. 
-    intro Hfalse. contradiction.
-  + simpl. fold @domain. intro Hdespl.
-    pose proof (Decidable.not_or (k = key) (In key (domain tail)) Hdespl) as Hindomain.
-    destruct Hindomain as [Hkkey Hdomaintail].
-    rewrite eqb_sym.
-    rewrite <- eqb_neq in Hkkey.
-    rewrite -> Hkkey.
-    apply IHtail in Hdomaintail.
-    assumption.
-Qed.
 
 
 
@@ -372,17 +35,17 @@ Inductive sfs_val : Type :=
   | SFSconst (v: EVMWord)
   | SFSname (name: string)
   | SFSbinop (op: OpCode) (name1 name2: string).
-  (* SFSuop y SFSterop *)
+  (* SFSuop & SFSterop for unary and ternary operations, if needed *)
   
 Definition sfs_map := map sfs_val.
 
 Inductive sfs : Type := 
-  SFS (abs: abstract_stack) (map: sfs_map).
+  SFS (absi: abstract_stack) (abso: abstract_stack) (sfsmap: sfs_map).
 
 (* Initial stack and SFS map contains disjoint symbols *)
 Definition disjoint_stack_sfs (stack: map EVMWord) (csfs: sfs) : Prop :=
 match csfs with 
-  | SFS abs sfsmap => disjoint (domain stack) (domain sfsmap)
+  | SFS absi abso sfsmap => disjoint (domain stack) (domain sfsmap)
 end.
 
 
@@ -472,8 +135,8 @@ Definition abs_eval_push (arg: word 5) (word: EVMWord) (curr_sfs: sfs) (fresh_st
 match fresh_stack_names with
  | nil => None
  | next_stack_name::rest_stack_names => match curr_sfs with
-                                         | SFS sfs_stack sfs_map => let value := pushWordPass word (wordToNat arg + 1) in
-                                                                    Some (SFS (next_stack_name::sfs_stack) 
+                                         | SFS absi abso sfs_map => let value := pushWordPass word (wordToNat arg + 1) in
+                                                                    Some (SFS absi (next_stack_name::abso) 
                                                                               (update sfs_map next_stack_name (SFSconst value)), 
                                                                           rest_stack_names)
                                          end
@@ -482,8 +145,8 @@ end.
 Definition abs_eval_pop (curr_sfs: sfs) (fresh_stack_names: list string)
   : option (sfs * list string) :=
 match curr_sfs with
- | SFS sfs_stack sfs_map => match sfs_stack with
-                             | top::r => Some ((SFS r sfs_map), fresh_stack_names)
+ | SFS absi abso sfs_map => match abso with
+                             | top::r => Some ((SFS absi r sfs_map), fresh_stack_names)
                              | nil => None
                             end
 end.
@@ -495,9 +158,9 @@ match fresh_stack_names with
  | nil => None
  | next_stack_name::rest_stack_names =>
      match curr_sfs with
-      | SFS sfs_stack sfs_map =>
-          match sfs_stack with
-           | s0::s1::rstack => Some (SFS (next_stack_name::rstack) 
+      | SFS absi abso sfs_map =>
+          match abso with
+           | s0::s1::rstack => Some (SFS absi (next_stack_name::rstack) 
                                          (update sfs_map next_stack_name (SFSbinop oper s0 s1)),
                                      rest_stack_names)
            | _ => None
@@ -505,8 +168,8 @@ match fresh_stack_names with
      end
 end.
 
-Compute abs_eval_binary (SimplePriceOpcodeMk ADD) (SFS ("s0"::"s1"::nil) empty_map) ("nueva pos"::"otra mas"::nil).
-Compute abs_eval_binary (SimplePriceOpcodeMk SUB) (SFS ("s0"::"s1"::"s2"::nil) empty_map) ("nueva pos"::"name2"::nil).
+Compute abs_eval_binary (SimplePriceOpcodeMk ADD) (SFS ("s0"::"s1"::nil) ("s0"::"s1"::nil) empty_map) ("nueva pos"::"otra mas"::nil).
+Compute abs_eval_binary (SimplePriceOpcodeMk SUB) (SFS ("s0"::"s1"::"s2"::nil) ("s0"::"s1"::"s2"::nil) empty_map) ("nueva pos"::"name2"::nil).
 
 
 (* Function to evaluate an operation in a SFS *)
@@ -531,8 +194,8 @@ match oper with
 end.
 
 Check (abs_eval_op).
-Compute abs_eval_op (SimplePriceOpcodeMk ADD) (SFS ("s0"::"s1"::nil) empty_map) ("nueva pos"::"otra mas"::nil).
-Compute abs_eval_op (SimplePriceOpcodeMk SUB) (SFS ("s0"::"s1"::nil) empty_map) ("nueva pos"::"otra mas"::nil).
+Compute abs_eval_op (SimplePriceOpcodeMk ADD) (SFS ("s0"::"s1"::nil) ("s0"::"s1"::nil) empty_map) ("nueva pos"::"otra mas"::nil).
+Compute abs_eval_op (SimplePriceOpcodeMk SUB) (SFS ("s0"::"s1"::nil) ("s0"::"s1"::nil) empty_map) ("nueva pos"::"otra mas"::nil).
 
 
 Fixpoint abstract_eval_aux (program: list OpCode) (curr_sfs: sfs) (fresh_stack_names: list string)
@@ -549,7 +212,7 @@ Definition abstract_eval (program: list OpCode)
   : option sfs :=
 let ins := create_abs_stack_name 10 "s" in (* The 10 is fixed... *)
 let outs := create_abs_stack_name StackLen "e" in (* generates 'StackLen' names*)
-match abstract_eval_aux program (SFS ins empty_map) outs with
+match abstract_eval_aux program (SFS ins ins empty_map) outs with
  | None => None
  | Some (final_sfs, _) => Some final_sfs
 end.
@@ -670,7 +333,7 @@ match d with
  | S d' => match lookup concrete_stack symbol with
             | Some value => Some value
             | None => match spec with 
-                       | SFS _ sfsm => match lookup sfsm symbol with
+                       | SFS _ _ sfsm => match lookup sfsm symbol with
                                         | Some (SFSconst v) => Some v
                                         | Some (SFSbinop oper name1 name2) => 
                                             match (evaluate_sfs_from_map d' concrete_stack spec name1,
@@ -686,36 +349,36 @@ match d with
 end.
 
 
-Lemma eval_more_steps: forall (d: nat) (stack: map EVMWord) (ini_abs: abstract_stack) 
-(ini_sfs_map: sfs_map) (symbol: string) (val: EVMWord),
-evaluate_sfs_from_map d stack (SFS ini_abs ini_sfs_map) symbol = Some val
--> evaluate_sfs_from_map (S d) stack (SFS ini_abs ini_sfs_map) symbol = Some val.
+Lemma eval_more_steps: forall (d: nat) (stack: map EVMWord) (absi abso: abstract_stack) 
+(sfs_map: sfs_map) (symbol: string) (val: EVMWord),
+evaluate_sfs_from_map d stack (SFS absi abso sfs_map) symbol = Some val
+-> evaluate_sfs_from_map (S d) stack (SFS absi abso sfs_map) symbol = Some val.
 Proof.
 intro d. induction d as [ | d' IH].
- - intros stack ini_abs ini_sfs_map symbol val.
+ - intros stack absi abso sfs_map symbol val.
    unfold evaluate_sfs_from_map. intro Hnonesome. discriminate.
- - intros stack ini_abs ini_sfs_map symbol val.
+ - intros stack absi abso sfs_map symbol val.
    remember (S d') as succdp eqn: Heqsuccdp. (* Defines succdp = S d', useful for unfolding *)
    rewrite -> Heqsuccdp at 1.
    unfold evaluate_sfs_from_map.
    destruct (lookup stack symbol) as [v | ] eqn: eqlookupstackvalue; try trivial.
-   destruct (lookup ini_sfs_map symbol) as [v | ] eqn: eqlookupmapvalue; try trivial.
+   destruct (lookup sfs_map symbol) as [v | ] eqn: eqlookupmapvalue; try trivial.
    destruct v as [value|name|op name1 name2] eqn: Hv.
    + trivial.
    + fold evaluate_sfs_from_map.
      rewrite -> Heqsuccdp.
-     pose proof (IH stack ini_abs ini_sfs_map name val) as IHspec.
+     pose proof (IH stack absi abso sfs_map name val) as IHspec.
      rewrite -> Heqsuccdp in IHspec.
      assumption.
    + fold evaluate_sfs_from_map.
-     destruct (evaluate_sfs_from_map d' stack (SFS ini_abs ini_sfs_map) name1) 
+     destruct (evaluate_sfs_from_map d' stack (SFS absi abso sfs_map) name1) 
        as [v1|] eqn: Hevalname1.
-     * destruct (evaluate_sfs_from_map d' stack (SFS ini_abs ini_sfs_map) name2) 
+     * destruct (evaluate_sfs_from_map d' stack (SFS absi abso sfs_map) name2) 
           as [v2|] eqn: Hevalname2.
-       -- pose proof (IH stack ini_abs ini_sfs_map name1 v1) as IHspecname1.
+       -- pose proof (IH stack absi abso sfs_map name1 v1) as IHspecname1.
           apply IHspecname1 in Hevalname1.
           rewrite -> Hevalname1.
-          pose proof (IH stack ini_abs ini_sfs_map name2 v2) as IHspecname2.
+          pose proof (IH stack absi abso sfs_map name2 v2) as IHspecname2.
           apply IHspecname2 in Hevalname2.
           rewrite -> Hevalname2.
           trivial.
@@ -754,18 +417,18 @@ end.
 
 
 Compute (let init_map := ("s0", natToWord WLen 6)::("s1", (natToWord WLen 5))::nil in 
-         let spec := SFS nil (("e0", SFSbinop (SimplePriceOpcodeMk ADD) "s0" "s1")::nil) in 
+         let spec := SFS nil nil (("e0", SFSbinop (SimplePriceOpcodeMk ADD) "s0" "s1")::nil) in 
          safeWordToNat (evaluate_sfs_from_map StackLen init_map spec "s1")).
 Compute (let init_map := ("s0", natToWord WLen 6)::("s1", (natToWord WLen 5))::nil in 
-         let spec := SFS nil (("e0", SFSbinop (SimplePriceOpcodeMk ADD) "s0" "s1")::nil) in 
+         let spec := SFS nil nil (("e0", SFSbinop (SimplePriceOpcodeMk ADD) "s0" "s1")::nil) in 
          safeWordToNat (evaluate_sfs_from_map StackLen init_map spec "e0")).
 Compute (let init_map := ("s0", natToWord WLen 6)::("s1", (natToWord WLen 5))::("s2", (natToWord WLen 2))::nil in 
-         let spec := SFS nil (("e0", SFSbinop (SimplePriceOpcodeMk ADD) "s0" "s1")::
+         let spec := SFS nil nil (("e0", SFSbinop (SimplePriceOpcodeMk ADD) "s0" "s1")::
                               ("e1", SFSbinop (SimplePriceOpcodeMk MUL) "e0" "s2")::nil) in 
          safeWordToNat (evaluate_sfs_from_map StackLen init_map spec "e1")).
 Compute (let init_map := ("s0", natToWord WLen 6)::("s1", (natToWord WLen 5))::
                          ("s2", (natToWord WLen 2))::("s3", (natToWord WLen 2))::nil in 
-         let spec := SFS nil (("e0", SFSbinop (SimplePriceOpcodeMk ADD) ("s0") ("s1"))::
+         let spec := SFS nil nil (("e0", SFSbinop (SimplePriceOpcodeMk ADD) ("s0") ("s1"))::
                               ("e1", SFSbinop (SimplePriceOpcodeMk MUL) ("e0") ("s2"))::
                               ("e2", SFSbinop (SimplePriceOpcodeMk SUB) ("e1") ("s3"))::nil) in 
          safeWordToNat (evaluate_sfs_from_map StackLen init_map spec "e2")).
@@ -790,14 +453,14 @@ reflexivity. Qed.
 (* Two SFS specifications are the same if given a concrete stack, they evaluate their
    abstract symbols to the same EVM values (EVMWord) *)
 Fixpoint sfs_equiv_concrete_values_aux (concrete_stack: map EVMWord) 
-  (abs1: abstract_stack) (sfsmap1: sfs_map) (abs2: abstract_stack) (sfsmap2: sfs_map) : bool :=
-match (abs1, abs2) with
+  (absi1 absi2 abso1 abso2: abstract_stack) (sfsmap1 sfsmap2: sfs_map) : bool :=
+match (abso1, abso2) with
   | (nil, nil) => true  
   | (symb1::r1, symb2::r2) => 
-      let v1 := evaluate_sfs_from_map 1024 concrete_stack (SFS abs1 sfsmap1) symb1 in
-      let v2 := evaluate_sfs_from_map 1024 concrete_stack (SFS abs2 sfsmap2) symb2 in
+      let v1 := evaluate_sfs_from_map 1024 concrete_stack (SFS absi1 abso1 sfsmap1) symb1 in
+      let v2 := evaluate_sfs_from_map 1024 concrete_stack (SFS absi2 abso2 sfsmap2) symb2 in
       match (v1, v2) with
-       | (Some w1, Some w2) => andb (weqb w1 w2) (sfs_equiv_concrete_values_aux concrete_stack r1 sfsmap1 r2 sfsmap2)
+       | (Some w1, Some w2) => andb (weqb w1 w2) (sfs_equiv_concrete_values_aux concrete_stack absi1 r1 absi2 r2 sfsmap1 sfsmap2)
        | _ => false
       end
   | _ => false
@@ -808,7 +471,7 @@ end.
    stack position to the same concrete value (wrt. the concrete stack) *)
 Definition sfs_equiv_concrete_values (concrete_stack: map EVMWord) (spec1 spec2: sfs) : bool :=
 match (spec1, spec2) with
- | (SFS abs1 sfsmap1, SFS abs2 sfsmap2) => sfs_equiv_concrete_values_aux concrete_stack abs1 sfsmap1 abs2 sfsmap2
+ | (SFS absi1 abso1 sfsmap1, SFS absi2 abso2 sfsmap2) => sfs_equiv_concrete_values_aux concrete_stack absi1 absi2 abso1 abso2 sfsmap1 sfsmap2
 end.
 Check sfs_equiv_concrete_values.
 
@@ -887,563 +550,4 @@ end
 ).
 
 
-
-(*************
-  POINTS-TO symbol to constant
- *************)
-
-(* Checks if the mapping of the 'label' in the 'smap' is the constant 'value' in one step *)
-Definition points_to_const (label: string) (smap: sfs_map) (value: EVMWord) : bool :=
-match lookup smap label with
- | Some (SFSconst val) => weqb val value
- | _ => false
-end.
-
-Compute (
-abstract_eval (SimplePriceOpcodeMk (PUSH (natToWord 5 0) WZero)::
-               SimplePriceOpcodeMk ADD::
-               nil)).
-
-Compute (
-match abstract_eval (SimplePriceOpcodeMk (PUSH (natToWord 5 0) WZero)::
-                     SimplePriceOpcodeMk ADD::
-                     nil) with
- | Some (SFS abs smap) => Some (points_to_const "e0" smap WZero)
- | _ => None
-end
-).
-
-
-Lemma points_to_then_eval: forall (d:nat) (symb: string) (abs: abstract_stack)
-      (csfs_map: sfs_map) (value val: EVMWord) (concrete_stack: map EVMWord),
- (points_to_const symb csfs_map value) = true
- -> lookup concrete_stack symb = None
- -> evaluate_sfs_from_map d concrete_stack (SFS abs csfs_map) symb = Some val 
- -> val = value.
-Proof. 
- intros d symb abs csfs_map value val concrete_stack.
- unfold points_to_const.
- destruct (lookup csfs_map symb) as [s|] eqn: eqlookup.
- + destruct s as [ | name | ] eqn: eqs.
-   - unfold evaluate_sfs_from_map. destruct d as [ | d'] eqn: eqd.
-     * intros Heq HNonesome. discriminate.
-     * intros Heq Hlookup. rewrite -> Hlookup.
-       rewrite -> eqlookup.
-       destruct d' as [ | d''] eqn: eqd'.
-       ++ intros Hvval. injection Hvval.
-          injection Hvval.
-          intro eqvval.
-          apply weqb_true_iff in Heq.
-          rewrite -> Heq. intros Hvalueval.
-          symmetry. assumption.
-       ++ intros Hvval. injection Hvval.
-          injection Hvval.
-          intro eqvval.
-          apply weqb_true_iff in Heq.
-          rewrite -> Heq. intros Hvalueval.
-          symmetry. assumption.
-  - destruct (lookup csfs_map name) eqn: eqlookup2.
-    * intros falsetrue. discriminate.
-    * intros falsetrue. discriminate.
-  - intros falsetrue. discriminate.
- + intros falsetrue. discriminate.
-Qed.
-
-
-(* If points_to detect that a symbol points to a constant in the SFS, then it cannot 
-   appear in the stack because they are disjoint *)
-Lemma points_to_not_in_stack: forall (stack: map EVMWord) (ini_abs: abstract_stack) 
-                             (ini_sfs_map: sfs_map) (name: string) (val: EVMWord),
-disjoint_stack_sfs stack (SFS ini_abs ini_sfs_map)
--> points_to_const name ini_sfs_map val = true
--> lookup stack name = None.
-Proof.
-intros stack ini_abs ini_sfs_map name val.
-unfold disjoint_stack_sfs.
-intro Hdisjoint.
-unfold points_to_const.
-destruct (lookup ini_sfs_map name) as [valname|] eqn: Hlookupmap;
-  try (intro Hfalse; discriminate).
-destruct valname as [constname|rname|op name1 name2] eqn: Hvalname;
-  try (intro Hfalse; discriminate).
-pose proof (@lookup_then_key_in_domain sfs_val ini_sfs_map name
-  (SFSconst constname) Hlookupmap) as Hname_in_sfsmap.
-pose proof (disjoint_then_not_in (domain stack) (domain ini_sfs_map)
-  name Hdisjoint).
-pose proof (disjoint_sym (domain stack) (domain ini_sfs_map) Hdisjoint)
-  as Hdisjoint_sym.
-pose proof (disjoint_then_not_in (domain ini_sfs_map) (domain stack)
-  name Hdisjoint_sym Hname_in_sfsmap) as Hname_not_in_stack.
-intro Heqconst.
-pose proof (@not_in_domain_then_lookup_none EVMWord stack name
-  Hname_not_in_stack) as Hlookup_none.
-assumption.
-Qed.
-
-
-
-(**************
-  OPTIMIZATION X+0 -> X
- **************)
-
-(* ADD(X, 0) -> X and ADD(0, X) -> X *)
-Definition optimize_add_zero (s: sfs) (var: string) : option sfs :=
-match s with
- | SFS abs smap => 
-     match lookup smap var with
-      | Some (SFSbinop (SimplePriceOpcodeMk ADD) a b) =>
-          if points_to_const a smap WZero then Some (SFS abs (update smap var (SFSname b)))
-          else if points_to_const b smap WZero then Some (SFS abs (update smap var (SFSname a)))
-          else None
-      | _ => None
-     end
-end.
-
-Compute (
-match abstract_eval (SimplePriceOpcodeMk (PUSH (natToWord 5 0) WZero)::
-                     SimplePriceOpcodeMk ADD::
-                     nil) with
- | Some (SFS abs smap) => optimize_add_zero (SFS abs smap) "e1"
- | _ => None
-end
-).
-
-Compute (
-match abstract_eval (SimplePriceOpcodeMk (PUSH (natToWord 5 0) (natToWord WLen 15))::
-                     SimplePriceOpcodeMk (PUSH (natToWord 5 0) WZero)::
-                     SimplePriceOpcodeMk ADD::
-                     nil) with
- | Some (SFS abs smap) => optimize_add_zero (SFS abs smap) "e2"
- | _ => None
-end
-).
-
-
-Lemma optimize_add_zero_same_abs: forall (symb: string)
-      (ini_abs opt_abs: abstract_stack) (ini_sfs_map opt_sfs_map: sfs_map), 
-optimize_add_zero (SFS ini_abs ini_sfs_map) symb = Some (SFS opt_abs opt_sfs_map) ->
-ini_abs = opt_abs.
-Proof.
-intros symb ini_abs opt_abs ini_sfs_map opt_sfs_map.
-unfold optimize_add_zero.
-destruct (lookup ini_sfs_map symb) as [sfsvalue|] eqn:eqlookupsymb; try discriminate.
-destruct sfsvalue as [ | |op name1 name2] eqn: eqsfsvalue; try discriminate.
-destruct op as [ | | |instr] eqn: eqop; try discriminate.
- (* Tries to apply discrimiante for all instructions 'op', that succeeds except 
-    for SimplePriceOpcodeMk *)
-destruct instr eqn: eqinstr; try discriminate. 
-(* Tries to apply discrimiante for all simple instructions 'instr', that succeeds except 
-   for ADD *)
-destruct (points_to_const name1 ini_sfs_map WZero) eqn: eqhaszeroa.
- - intro Hini_opt. injection Hini_opt. intros Hopt_map Hopt_abs. assumption.
- - destruct (points_to_const name2 ini_sfs_map WZero) eqn: eqhaszerob; try discriminate.
-   intro Hini_opt. injection Hini_opt. intros Hopt_map Hopt_abs. assumption.
-Qed.   
-Check (optimize_add_zero_same_abs).
-
-
-
-Lemma optimize_add_zero_symb_same_value_init: 
- forall (d: nat) (concrete_stack: map EVMWord) (ini_sfs opt_sfs: sfs) (symb: string)
- (c: EVMWord),
- lookup concrete_stack symb = Some c
- -> optimize_add_zero ini_sfs symb = Some opt_sfs
- -> evaluate_sfs_from_map d concrete_stack ini_sfs symb =
-    evaluate_sfs_from_map d concrete_stack opt_sfs symb.
-Proof.
- intros d stack ini_sfs opt_sfs symb c Hlookup HoptSome.
- unfold evaluate_sfs_from_map.
- unfold evaluate_sfs_from_map. destruct d as [ | d'] eqn:eqd; try reflexivity.
- rewrite -> Hlookup. reflexivity.
-Qed.
-
-
-(* Evaluating X+0 = X in EVM words *)
-Lemma evalADDzero: forall (e: EVMWord),
- evaluate_concrete_element (SimplePriceOpcodeMk ADD) (WZero :: e :: nil) = Some e.
-Proof.
- intros e. unfold evaluate_concrete_element. simpl.
- unfold WZero.
- rewrite -> wplus_wzero_2.
- reflexivity.
- Qed.
- 
-(* Evaluating 0+X = X in EVM words *) 
-Lemma evalADDzero2: forall (e: EVMWord),
- evaluate_concrete_element (SimplePriceOpcodeMk ADD) (e :: WZero :: nil) = Some e.
-Proof.
- intros e. unfold evaluate_concrete_element. simpl.
- unfold WZero.
- rewrite -> wplus_wzero_1.
- reflexivity.
- Qed.
-
-
-(* If you can apply  the X+0 optimization in symbol 'symb', then it must be mapped
-   to a some addition name1 + name2 in the SFS *)
-Lemma opt_add_zero_then_binopADD: forall (ini_abs opt_abs: abstract_stack) 
-   (ini_sfs_map opt_sfs_map: sfs_map) (symb: string),
-optimize_add_zero (SFS ini_abs ini_sfs_map) symb = Some (SFS opt_abs opt_sfs_map) ->
-exists (name1 name2: string), lookup ini_sfs_map symb = Some (SFSbinop 
-  (SimplePriceOpcodeMk ADD) name1 name2).
-Proof.
-intros ini_abs opt_abs ini_sfs_map opt_sfs_map symb.
-unfold optimize_add_zero.
-destruct (lookup ini_sfs_map symb) as [symb_expr|] eqn: Hlookupsymb;
-  try (intro Hfalse; discriminate).
-destruct symb_expr as [value|name|op n1 n2]; try (intro Hfalse; discriminate).
-destruct op as [ | | | oper]; try (intro Hfalse; discriminate).
-destruct oper; try (intro Hfalse; discriminate).
-destruct (points_to_const n1 ini_sfs_map WZero) eqn: Hpointsto_n1.
-- intro Hopt. exists n1. exists n2. reflexivity.
-- destruct (points_to_const n2 ini_sfs_map WZero) eqn: Hpointsto_name2; 
-    try (intro Hfalse; discriminate).
-  intro Hopt. exists n1. exists n2. reflexivity.
-Qed.  
-
-
-(* If you can apply the X+0 optimization in symbol 'symb', then the new SFS mapping
-   is just the original one but replacing 'symb' *)
-Lemma opt_add_zero_only_affects_symbol: forall (ini_abs opt_abs: abstract_stack) 
-   (ini_sfs_map opt_sfs_map: sfs_map) (symb: string),
-optimize_add_zero (SFS ini_abs ini_sfs_map) symb = Some (SFS opt_abs opt_sfs_map) ->
-exists (sfsexpr: sfs_val), opt_sfs_map = update ini_sfs_map symb sfsexpr.
-Proof.
-intros ini_abs opt_abs ini_sfs_map opt_sfs_map symb.
-unfold optimize_add_zero.
-destruct (lookup ini_sfs_map symb) as [symb_expr|] eqn: Hlookupsymb;
-  try (intro Hfalse; discriminate).
-destruct symb_expr as [value|name|op n1 n2]; try (intro Hfalse; discriminate).
-destruct op as [ | | | oper]; try (intro Hfalse; discriminate).
-destruct oper; try (intro Hfalse; discriminate).
-destruct (points_to_const n1 ini_sfs_map WZero) eqn: Hpointsto_n1.
-- intro Hopt. injection Hopt. intro Hopt_sfs_map. intro Hopt_abs. 
-  rewrite <- Hopt_sfs_map. exists (SFSname n2). reflexivity.
-- destruct (points_to_const n2 ini_sfs_map WZero) eqn: Hpointsto_name2; 
-    try (intro Hfalse; discriminate).
-  intro Hopt. injection Hopt. intro Hopt_sfs_map. intro Hopt_abs. 
-  rewrite <- Hopt_sfs_map. exists (SFSname n1). reflexivity.
-Qed.
-
-
-(* If you can apply the X+0 optimization in symbol 'symb', then the SFS mapping
-   contained a name1 + name2 where
-   a) name1 points to WZero and [symb |-> name2] in the new SFS mapping
-   b) name1 does not point to WZero, name2 points to WZero and [symb |-> name1] 
-        in the new SFS mapping *)
-Lemma opt_add_zero_then_pointsto: forall (ini_abs opt_abs: abstract_stack) 
-      (ini_sfs_map opt_sfs_map: sfs_map)
-      (symb name1 name2: string),
-optimize_add_zero (SFS ini_abs ini_sfs_map) symb = Some (SFS opt_abs opt_sfs_map) ->
-lookup ini_sfs_map symb = 
-  Some (SFSbinop (SimplePriceOpcodeMk ADD) name1 name2) ->
-(points_to_const name1 ini_sfs_map WZero = true /\
- opt_sfs_map = update ini_sfs_map symb (SFSname name2)) 
-\/ 
-(points_to_const name1 ini_sfs_map WZero = false /\
- points_to_const name2 ini_sfs_map WZero = true /\
- opt_sfs_map = update ini_sfs_map symb (SFSname name1)).
-Proof.
-intros ini_abs opt_abs ini_sfs_map opt_sfs_map symb name1 name2.
-unfold optimize_add_zero.
-destruct (lookup ini_sfs_map symb) as [symb_expr|] eqn: Hlookupsymb;
-  try (intro Hfalse; discriminate).
-destruct symb_expr as [value|name|op n1 n2]; try (intro Hfalse; discriminate).
-destruct op as [ | | | oper]; try (intro Hfalse; discriminate).
-destruct oper; try (intro Hfalse; discriminate).
-destruct (points_to_const n1 ini_sfs_map WZero) eqn: Hpointsto_n1.
-- intro Hopt_sfs. injection Hopt_sfs. intro Hopt_sfs_map. intro Hopt_abs.
-  intro Hsfsexpr. injection Hsfsexpr. intros Hn2 Hn1.
-  left.
-  symmetry in Hopt_sfs_map.
-  rewrite <- Hn1.
-  rewrite <- Hn2.
-  split; try assumption.
-- destruct (points_to_const n2 ini_sfs_map WZero) eqn: Hpointsto_n2; 
-    try (intro Hfalse; discriminate).
-  intro Hopt_sfs. injection Hopt_sfs. intro Hopt_sfs_map. intro Hopt_abs.
-  intro Hsfsexpr. injection Hsfsexpr. intros Hn2 Hn1.
-  right.
-  symmetry in Hopt_sfs_map.
-  rewrite <- Hn1.
-  rewrite <- Hn2.
-  split; try assumption.
-  split; try assumption.
-Qed.
-
-
-(* In the add-zero optimization of symbol 'symb', all the other symbols points to the 
-   SFS expression *)
-Lemma optimize_add_zero_same_but_symb: 
- forall (symb symb2: string)
- (ini_abs opt_abs: abstract_stack) (ini_sfs_map opt_sfs_map: sfs_map), 
- symb =? symb2 = false
- -> optimize_add_zero (SFS ini_abs ini_sfs_map) symb = Some (SFS opt_abs opt_sfs_map) 
- -> lookup ini_sfs_map symb2 = lookup opt_sfs_map symb2.
-Proof.
- intros symb symb2 ini_abs opt_abs ini_sfs_map opt_sfs_map HSymb Hopt.
- pose proof (opt_add_zero_only_affects_symbol ini_abs opt_abs ini_sfs_map
-    opt_sfs_map symb Hopt) as Haffect_ex.
- destruct Haffect_ex as [sfsval Haffect].
- rewrite -> Haffect.
- pose proof (update_lookup_diff sfs_val ini_sfs_map symb symb2 sfsval
-   HSymb) as Hlookup.
- rewrite -> Hlookup.
- reflexivity.
-Qed.
-
-
-
-Lemma pointsto_and_none_then_0_steps: forall (d: nat) (ini_abs: abstract_stack)
-  (ini_sfs_map: sfs_map) (stack: map EVMWord) (val: EVMWord) (symbol: string),
-disjoint_stack_sfs stack (SFS ini_abs ini_sfs_map) ->
-points_to_const symbol ini_sfs_map val = true ->
-evaluate_sfs_from_map d stack (SFS ini_abs ini_sfs_map) symbol = None ->
-d = 0.
-Proof.
-intros d ini_abs ini_sfs_map stack val symbol Hdisjoint Hpointsto Heval.
-(*remember Hpointsto as Hpointsto_orig eqn: eqpointsto. *)
-(*unfold points_to_const in Hpointsto.*)
-destruct (lookup ini_sfs_map symbol) as [sfs_expr|] eqn: eqlookup.
-- destruct (sfs_expr) as [const|name|name1 name2] eqn: eqsfs_expr.
-  * (* SFSconst *)
-    unfold evaluate_sfs_from_map in Heval.
-    destruct d as [|d']; try reflexivity.
-    pose proof (points_to_not_in_stack stack ini_abs ini_sfs_map symbol val
-      Hdisjoint Hpointsto) as Hnotinstack.
-    rewrite -> Hnotinstack in Heval.
-    rewrite -> eqlookup in Heval.
-    discriminate.
-  * (* SFSname *)
-    unfold points_to_const in Hpointsto.
-    rewrite -> eqlookup in Hpointsto.
-    discriminate.
-  * (* SFSbinop oper name1 name2 *) 
-    unfold points_to_const in Hpointsto.
-    rewrite -> eqlookup in Hpointsto.
-    discriminate.
-- unfold points_to_const in Hpointsto.
-  rewrite -> eqlookup in Hpointsto.
-  discriminate.
-Qed.
-
-
-
-(* 
-   MAIN THEOREM FOR THE X+0 OPTIMIZATION 
-   Evaluating a symbol in the original SFS returns the same as evaluating
-   it in the optimized SFS 
-*)
-Theorem optimize_add_zero_correct: forall (d: nat) 
-        (concrete_stack: map EVMWord) (ini_sfs opt_sfs: sfs) 
-        (symbol_opt symbol: string),
-disjoint_stack_sfs concrete_stack ini_sfs ->
-optimize_add_zero ini_sfs symbol_opt = Some opt_sfs ->
-evaluate_sfs_from_map d concrete_stack ini_sfs symbol = 
-evaluate_sfs_from_map d concrete_stack opt_sfs symbol.
-Proof.
-intro d. induction d as [|d' IH].
-- intros stack ini_sfs opt_sfs symbol_opt symbol Hdisjoint Hopt.
-  reflexivity.
-- intros stack ini_sfs opt_sfs symbol_opt symbol Hdisjoint Hopt.
-  destruct ini_sfs as [ini_abs ini_sfs_map] eqn: eqini_sfs.
-  destruct opt_sfs as [opt_abs opt_sfs_map] eqn: eqopt_sfs.
-  unfold evaluate_sfs_from_map.
-  destruct (lookup stack symbol) as [valstack|] eqn: eqlookupstack; try trivial.
-  (* lookup stack symbol = None *)
-  destruct (symbol_opt =? symbol) eqn: eqsymbolopt.
-  + (* Evaluating the same symbol that was optimized *)
-    pose proof (opt_add_zero_then_binopADD ini_abs opt_abs ini_sfs_map
-       opt_sfs_map symbol_opt Hopt) as Hlookup_opt_symb_exists.
-    destruct Hlookup_opt_symb_exists as [name1 Hlookup_opt_symb_exists2].
-    destruct Hlookup_opt_symb_exists2 as [name2 Hlookup_opt_symb].
-    apply -> eqb_eq in eqsymbolopt.
-    rewrite -> eqsymbolopt in Hlookup_opt_symb.
-    rewrite -> Hlookup_opt_symb.
-    fold evaluate_sfs_from_map.
-    rewrite -> eqsymbolopt in Hopt.
-    pose proof (opt_add_zero_then_pointsto ini_abs opt_abs ini_sfs_map 
-       opt_sfs_map symbol name1 name2 Hopt Hlookup_opt_symb) as Hoptimize_cases.
-    destruct Hoptimize_cases as [Hoptimize_name1 | Hoptimize_name2].
-    * destruct Hoptimize_name1 as [Hpointsto_name1 Hlookup_opt_symbol].
-      destruct (evaluate_sfs_from_map d' stack (SFS ini_abs ini_sfs_map) name1)
-         as [val1 | ] eqn: eqevalname1.
-      -- destruct (evaluate_sfs_from_map d' stack (SFS ini_abs ini_sfs_map) name2)
-            as [val2 |] eqn: eqevalname2.
-         ++ pose proof (points_to_not_in_stack stack ini_abs ini_sfs_map name1
-               WZero Hdisjoint Hpointsto_name1) as Hname1_not_in_stack.
-            pose proof (points_to_then_eval d' name1 ini_abs ini_sfs_map WZero 
-               val1 stack Hpointsto_name1 Hname1_not_in_stack eqevalname1) as Hval1_zero.
-            rewrite -> Hval1_zero.
-            rewrite -> evalADDzero.
-            rewrite -> Hlookup_opt_symbol.
-            pose proof (update_lookup sfs_val ini_sfs_map symbol 
-               (SFSname name2)) as Hlookup_symbol_opt.
-            rewrite -> Hlookup_symbol_opt.
-            rewrite <- Hlookup_opt_symbol.
-            rewrite <- eqopt_sfs.
-            rewrite <- eqini_sfs in Hdisjoint.
-            rewrite <- eqini_sfs in Hopt.
-            rewrite <- eqopt_sfs in Hopt.
-            rewrite <- eqini_sfs in eqevalname2.
-            pose proof (IH stack ini_sfs opt_sfs symbol name2
-               Hdisjoint Hopt) as IHspec.
-            rewrite <- IHspec.
-            rewrite -> eqevalname2.
-            reflexivity.
-         ++ pose proof (points_to_not_in_stack stack ini_abs ini_sfs_map name1
-               WZero Hdisjoint Hpointsto_name1) as Hname1_not_in_stack.
-            pose proof (points_to_then_eval d' name1 ini_abs ini_sfs_map WZero 
-               val1 stack Hpointsto_name1 Hname1_not_in_stack eqevalname1) as Hval1_zero.
-            rewrite -> Hlookup_opt_symbol.
-            pose proof (update_lookup sfs_val ini_sfs_map symbol 
-               (SFSname name2)) as Hlookup_symbol_opt.
-            rewrite -> Hlookup_symbol_opt.
-            rewrite <- Hlookup_opt_symbol.
-            rewrite <- eqopt_sfs.
-            rewrite <- eqini_sfs in Hdisjoint.
-            rewrite <- eqini_sfs in Hopt.
-            rewrite <- eqopt_sfs in Hopt.
-            rewrite <- eqini_sfs in eqevalname2.
-            pose proof (IH stack ini_sfs opt_sfs symbol name2
-               Hdisjoint Hopt) as IHspec.
-            rewrite <- IHspec.
-            rewrite -> eqevalname2.
-            reflexivity.
-      -- rewrite -> Hlookup_opt_symbol.
-         pose proof (pointsto_and_none_then_0_steps d' ini_abs ini_sfs_map stack
-           WZero name1 Hdisjoint Hpointsto_name1 eqevalname1) as Hdiszero.
-         pose proof (update_lookup sfs_val ini_sfs_map symbol 
-               (SFSname name2)) as Hlookup_symbol_opt.
-         rewrite -> Hlookup_symbol_opt.
-         rewrite -> Hdiszero.
-         reflexivity.
-    * destruct Hoptimize_name2 as [Hpointsto_name1 [Hpointsto_name2 Hlookup_opt_symbol]].
-      destruct (evaluate_sfs_from_map d' stack (SFS ini_abs ini_sfs_map) name1)
-         as [val1 | ] eqn: eqevalname1.
-      -- destruct (evaluate_sfs_from_map d' stack (SFS ini_abs ini_sfs_map) name2)
-            as [val2 |] eqn: eqevalname2.
-         ++ pose proof (points_to_not_in_stack stack ini_abs ini_sfs_map name2
-               WZero Hdisjoint Hpointsto_name2) as Hname2_not_in_stack.
-            pose proof (points_to_then_eval d' name2 ini_abs ini_sfs_map WZero 
-               val2 stack Hpointsto_name2 Hname2_not_in_stack eqevalname2) as Hval2_zero.
-            rewrite -> Hval2_zero.
-            rewrite -> evalADDzero2.
-            rewrite -> Hlookup_opt_symbol.
-            pose proof (update_lookup sfs_val ini_sfs_map symbol 
-               (SFSname name1)) as Hlookup_symbol_opt.
-            rewrite -> Hlookup_symbol_opt.
-            rewrite <- Hlookup_opt_symbol.
-            rewrite <- eqopt_sfs.
-            rewrite <- eqini_sfs in Hdisjoint.
-            rewrite <- eqini_sfs in Hopt.
-            rewrite <- eqopt_sfs in Hopt.
-            rewrite <- eqini_sfs in eqevalname1.
-            pose proof (IH stack ini_sfs opt_sfs symbol name1
-               Hdisjoint Hopt) as IHspec.
-            rewrite <- IHspec.
-            rewrite -> eqevalname1.
-            reflexivity.
-         ++ rewrite -> Hlookup_opt_symbol.
-            pose proof (pointsto_and_none_then_0_steps d' ini_abs ini_sfs_map stack
-              WZero name2 Hdisjoint Hpointsto_name2 eqevalname2) as Hdiszero.
-            pose proof (update_lookup sfs_val ini_sfs_map symbol 
-               (SFSname name1)) as Hlookup_symbol_opt.
-            rewrite -> Hlookup_symbol_opt.
-            rewrite -> Hdiszero.
-            reflexivity.
-      -- rewrite -> Hlookup_opt_symbol.
-         pose proof (update_lookup sfs_val ini_sfs_map symbol 
-               (SFSname name1)) as Hlookup_symbol_opt.
-         rewrite -> Hlookup_symbol_opt.
-         rewrite <- Hlookup_opt_symbol.
-         rewrite <- eqopt_sfs.
-         rewrite <- eqini_sfs in Hdisjoint.
-         rewrite <- eqini_sfs in Hopt.
-         rewrite <- eqopt_sfs in Hopt.
-         rewrite <- eqini_sfs in eqevalname1.
-         pose proof (IH stack ini_sfs opt_sfs symbol name1
-               Hdisjoint Hopt) as IHspec.
-         rewrite <- IHspec.
-         rewrite -> eqevalname1.
-         reflexivity.
-  + (* Evaluating a symbol different from the optimized one *)
-     destruct (lookup ini_sfs_map symbol) as [symbolexpr|] eqn: eqlookupsymbol.
-     * (* lookup ini_sfs_map = Some symbolexpr *)
-       pose proof (opt_add_zero_only_affects_symbol ini_abs opt_abs
-          ini_sfs_map opt_sfs_map symbol_opt Hopt) as Hupdate_opt.
-       destruct Hupdate_opt as [symb_sfs_expr Hopt_sfs_map].
-       rewrite -> Hopt_sfs_map.
-       rewrite -> update_lookup_diff; try assumption.
-       rewrite -> eqlookupsymbol.
-       (* Folding/unfolding of SFS to apply the IH *)
-       rewrite <- eqini_sfs in Hdisjoint.
-       rewrite <- eqini_sfs in Hopt.
-       rewrite <- eqopt_sfs in Hopt.
-       rewrite <- eqini_sfs.
-       rewrite <- Hopt_sfs_map.
-       rewrite <- eqopt_sfs.
-       destruct symbolexpr as [value|name|op name1 name2] eqn: eqsfsexpr.
-       -- reflexivity.
-       -- fold evaluate_sfs_from_map.
-          pose proof (IH stack ini_sfs opt_sfs symbol_opt name 
-            Hdisjoint Hopt) as IHname.
-          assumption.
-       -- fold evaluate_sfs_from_map.
-          pose proof (IH stack ini_sfs opt_sfs symbol_opt name1
-            Hdisjoint Hopt) as IHname1.
-          rewrite <- IHname1.
-          pose proof (IH stack ini_sfs opt_sfs symbol_opt name2
-            Hdisjoint Hopt) as IHname2.
-          rewrite <- IHname2.
-          reflexivity.
-     * (* lookup ini_sfs_map = None *)
-       pose proof (optimize_add_zero_same_but_symb symbol_opt symbol
-         ini_abs opt_abs ini_sfs_map opt_sfs_map eqsymbolopt Hopt) 
-         as Hlookup.
-       rewrite -> Hlookup in eqlookupsymbol.
-       rewrite -> eqlookupsymbol.
-       reflexivity.
-Qed.
-
-
-
-(************
-  OPTIMIZATION X*1 -> X
-  TODO
- ************)
-
-Definition WOne: EVMWord  := natToWord WLen 1.
-
-(* MUL(X, 1) -> X and MUL(1, X) -> X *)
-Definition optimize_mul_one (s: sfs) (var: string) : option sfs :=
-match s with
- | SFS abs smap => 
-     match lookup smap var with
-      | Some (SFSbinop (SimplePriceOpcodeMk MUL) a b) =>
-          if points_to_const a smap WOne then Some (SFS abs (update smap var (SFSname b)))
-          else if points_to_const b smap WOne then Some (SFS abs (update smap var (SFSname a)))
-          else None
-      | _ => None
-     end
-end.
-
-Compute (
-match abstract_eval (SimplePriceOpcodeMk (PUSH (natToWord 5 0) WOne)::
-                     SimplePriceOpcodeMk MUL::
-                     nil) with
- | Some (SFS abs smap) => optimize_mul_one (SFS abs smap) "e1"
- | _ => None
-end
-).
-
-Compute (
-match abstract_eval (SimplePriceOpcodeMk (PUSH (natToWord 5 0) (natToWord WLen 15))::
-                     SimplePriceOpcodeMk (PUSH (natToWord 5 0) WOne)::
-                     SimplePriceOpcodeMk MUL::
-                     nil) with
- | Some (SFS abs smap) => optimize_mul_one (SFS abs smap) "e2"
- | _ => None
-end
-).
 
