string_map.v
@@ -1,0 +1,365 @@
+(* Enrique Martin - Univ. Complutense de Madrid
+   Licensed under the GNU GENERAL PUBLIC LICENSE 3.0.
+
+   You may obtain a copy of the License at
+   https://www.gnu.org/licenses/gpl-3.0.txt
+*)
+
+
+Require Export Coq.Lists.List.
+Require Export Coq.Strings.Ascii.
+Require Export Coq.Strings.String.
+Open Scope string_scope.
+
+
+
+(* POSSIBLE IMPROVEMENTS:
+   - Use faster mappings. Instead of list (key, value) use AVL or RB trees as in evmModel (FMapAVL)
+   - Define domains as sets of strings
+*)
+
+
+(******************
+  LISTS OF STRINGS 
+ ******************)
+(* 'In' function for list of strings but returning a boolean *)
+Fixpoint In_list_str_eval (e: string) (l: list string) : bool :=
+match l with 
+  | nil => false
+  | v::tail => orb (v =? e) (In_list_str_eval e tail)
+end.
+
+(* In and In_list_str_eval are equivalent *)
+Lemma in_str_equiv_true: forall (e: string) (l: list string),
+  In e l <-> In_list_str_eval e l = true.
+Proof.
+intros e l. split. 
+ + induction l as [ | h t IH].
+   - intros H. apply in_nil in H. contradiction.
+   - intros H. destruct (eqb e h) eqn: elem_eq.
+     * unfold In_list_str_eval. rewrite eqb_sym in elem_eq. rewrite elem_eq. reflexivity.
+     * simpl. rewrite eqb_sym in elem_eq. rewrite elem_eq. simpl.
+       simpl in H. destruct H.
+       ++ rewrite <- eqb_eq in H. rewrite H in elem_eq.
+          discriminate elem_eq.
+       ++ apply IH in H. assumption.
+ + induction l as [ | h t IH].
+   - simpl. intros H. discriminate.
+   - unfold In_list_str_eval. destruct (h =? e) eqn:eq_eh.
+     * simpl. intros Htrue. rewrite eqb_sym in eq_eh. apply eqb_eq in eq_eh.
+       left. symmetry. assumption.
+     * simpl. fold In_list_str_eval. intros Hin. apply IH in Hin. right. assumption.
+Qed.
+
+
+
+(* In and In_list_str_eval are equivalent also in the negative case *)
+Lemma in_str_equiv_false: forall (e: string) (l: list string),
+  ~In e l <-> In_list_str_eval e l = false.
+Proof.
+intros e l. split. 
++ (* -> *)
+  induction l as [ | h t IH].
+  - intros Henotinnil. reflexivity.
+  - intros Henotin. destruct (eqb e h) eqn: elem_eq.
+    * simpl in Henotin.
+      pose proof (Decidable.not_or (h = e) (In e t) Henotin) as Henotin_despl.
+      destruct Henotin_despl as [Hehdiff Henotint].
+      rewrite <- eqb_eq in Henotin.
+      rewrite <- eqb_neq in Hehdiff.
+      rewrite -> eqb_sym in elem_eq.
+      rewrite elem_eq in Hehdiff.
+      discriminate.
+    * simpl in Henotin. simpl.
+      pose proof (Decidable.not_or (h = e) (In e t) Henotin) as Henotin_despl.
+      destruct Henotin_despl as [Hehdiff Henotint].
+      rewrite -> eqb_sym in elem_eq.
+      rewrite -> elem_eq. simpl.
+      apply IH in Henotint as Hfinal.
+      assumption.
++ (* <- *) induction l as [ | h t IH].
+  - intro Hinevalfalse. simpl. unfold not. trivial.
+  - intro Hinevalfalse. simpl in Hinevalfalse.
+    destruct (eqb e h) eqn: elem_eq.
+    * rewrite -> eqb_sym in elem_eq.
+      rewrite -> elem_eq in Hinevalfalse. simpl in Hinevalfalse.
+      discriminate.
+    * rewrite -> eqb_sym in elem_eq.
+      rewrite -> elem_eq in Hinevalfalse. simpl in Hinevalfalse.
+      apply IH in Hinevalfalse.
+      simpl.
+      unfold not.
+      intro Hin.
+      destruct Hin as [Heq|HInet].
+      ++ rewrite -> Heq in elem_eq.
+         rewrite -> eqb_refl in elem_eq.
+         discriminate.
+      ++ contradiction.
+Qed.
+
+(* In is decidable: In e l /\ ~ In e l
+   Useful to apply some lemma from library Coq.Logic.Decidable *)
+Lemma in_decidable: forall (e: string) (l: list string),
+Decidable.decidable (In e l).
+Proof.
+intros e l.
+unfold Decidable.decidable.
+rewrite in_str_equiv_true.
+destruct (In_list_str_eval e l) eqn: eqevalin.
+- left. reflexivity.
+- right. apply Bool.diff_false_true.
+Qed.
+
+
+(* In_list_string_eval is dedicable
+   Useful to apply some lemma from library Coq.Logic.Decidable *)
+Lemma in_list_str_eval_decidable: forall (e: string) (l: list string) (b:bool),
+Decidable.decidable (In_list_str_eval e l = b).
+Proof.
+intros e l b.
+unfold Decidable.decidable.
+destruct (In_list_str_eval e l) eqn: eqevalin.
+- destruct b eqn: eqb. 
+  + left. reflexivity.
+  + right. apply Bool.diff_true_false.
+- destruct b eqn: eqb. 
+  + right. apply Bool.diff_false_true.
+  + left. reflexivity.
+Qed.
+
+
+(* No element h of l1 appears in l2 *)
+Fixpoint not_in_list (l1 l2: list string) : Prop :=
+match l1 with
+  | nil => True
+  | h::t => ~ (In h l2) /\ (not_in_list t l2)
+end.
+
+Definition disjoint_eval (l1 l2: list string) : Prop :=
+(not_in_list l1 l2).
+
+Definition disjoint (l1 l2: list string) : Prop :=
+forall (x: string), In x l1 -> ~ In x l2.
+
+Lemma disjoint_extend: forall (l1 l2: list string) (elem: string),
+disjoint l1 l2 ->
+~ In elem l2 ->
+disjoint (elem::l1) l2.
+Proof.
+intros l1 l2 elem Hdisjoint Hnotin.
+unfold disjoint.
+intro e. simpl.
+rewrite <- eqb_eq.
+destruct (elem =? e) eqn: eqeleme.
+- simpl. rewrite -> eqb_eq in eqeleme.
+  rewrite <- eqeleme. intro Htrue. assumption.
+- unfold orb. intro He.
+  destruct He as [Hfalse | Heinl1].
+  + discriminate.
+  + unfold disjoint in Hdisjoint.
+    pose proof (Hdisjoint e) as Henotin.
+    apply Henotin in Heinl1.
+    assumption.
+Qed.
+
+Search In.
+
+
+Lemma disjoint_split: forall (l1 l2: list string) (elem: string),
+disjoint (elem::l1) l2 ->
+~ In elem l2 /\ disjoint l1 l2.
+Proof.
+intros l1 l2 elem.
+unfold disjoint.
+intros Himpl.
+split.
+- pose proof (Himpl elem).
+  pose proof (in_eq elem l1) as Helemincons.
+  apply H in Helemincons.
+  assumption.
+- intros y.
+  pose proof (Himpl y) as Himply.
+  intros Hyinl1.
+  pose proof (in_cons elem y l1) as Hyineleml1.
+  apply Hyineleml1 in Hyinl1.
+  apply Himply in Hyinl1.
+  assumption.
+Qed.
+
+
+
+Lemma disjoint_equiv: forall (l1 l2: list string),
+disjoint_eval l1 l2 <-> disjoint l1 l2.
+Proof.
+split.
+- (* -> *) 
+  induction l1 as [|h t IH].
+  + simpl. intro Htrue. unfold disjoint.
+    intro elem. simpl. intro Hfalse. contradiction.
+  + simpl. intros [Hnotinl2 Hdisjoint].
+    apply IH in Hdisjoint.
+    apply disjoint_extend; try assumption.
+- (* <- *)
+  induction l1 as [|h t IH].
+  + simpl. trivial. 
+  + simpl. intro Hdisjoint.
+    pose proof (disjoint_split t l2 h) as Hsplitdisjoint.
+    apply Hsplitdisjoint in Hdisjoint.
+    destruct Hdisjoint as [Hnotinl2 Hdisjointl2].
+    apply IH in Hdisjointl2.
+    split; try assumption.
+Qed.
+
+
+
+Lemma disjoint_sym: forall (l1 l2: list string),
+  (disjoint l1 l2) -> (disjoint l2 l1).
+Proof.
+intros l1 l2.
+unfold disjoint.
+intro Hdisjoint.
+intros elem Hxinl2.
+destruct (In_list_str_eval elem l1) eqn: Helem_in_l1.
+- rewrite <- in_str_equiv_true in Helem_in_l1.
+  pose proof (Hdisjoint elem Helem_in_l1). contradiction.
+- rewrite <- in_str_equiv_false in Helem_in_l1.
+  assumption.
+Qed.
+
+
+Lemma disjoint_then_not_in: forall (l m: list string) (name: string),
+disjoint l m ->
+In name l ->
+~ In name m.
+Proof.
+intros l m name Hdisjoint.
+unfold disjoint in Hdisjoint.
+pose proof (Hdisjoint name).
+assumption.
+Qed.
+
+
+
+
+
+(**********
+  MAPPINGS 
+ **********)
+
+(* Mapping as list of tuples with duplicates. Probably FMapAVL is better and faster, but we
+   need to define keys as OrderedType and I don't know how to do that *)
+Definition map (T : Type) : Type := list (string * T).
+Definition empty_map {A : Type} : map A := nil.
+Definition update {A : Type} (m : map A) (x : string) (v : A): map A :=
+  (x,v) :: m.
+Fixpoint lookup {A : Type} (m : map A) (x : string) : option A :=
+match m with
+  | nil => None
+  | (y,v)::tail => if x =? y then Some v else (lookup tail x)
+end.
+
+
+Fixpoint domain {A: Type} (m: map A) : list string :=
+match m with
+  | nil => nil
+  | (k,v)::tail => k::(domain tail)
+end.
+
+
+
+(* looking for a key after updating the map returns the inserted value *)
+Lemma update_lookup: forall (T: Type) (m:  map T) (key: string) (value: T),
+  lookup (update m key value) key = Some value.
+Proof.
+  intros T m key value.
+  unfold update. unfold lookup. destruct (key =? key) eqn: EqKey.
+  - reflexivity.
+  - rewrite -> (eqb_refl key) in EqKey. (* from Coq.Strings.String *)
+    discriminate.
+Qed.
+
+
+(* looking for a different key after updating the map is the same as looking in the
+   original map *)
+Lemma update_lookup_diff: forall (T: Type) (m:  map T) (key1 key2: string) (value: T),
+  key1 =? key2 = false -> lookup (update m key1 value) key2 = lookup m key2.
+Proof.
+  intros T m key1 key2 value HKey. unfold update. unfold lookup.
+  rewrite -> (eqb_sym key1 key2) in HKey. (* from Coq.Strings.String *)
+  rewrite HKey. reflexivity.
+Qed.
+
+
+Lemma lookup_then_key_in_domain: forall {A: Type} (m: map A) (key: string) 
+      (value: A),
+lookup m key = Some value -> In key (domain m).
+Proof.
+intros A m key value.
+induction m as [ | pair tail].
+- simpl. intro Hfalse. discriminate.
+- unfold lookup.
+  destruct (pair) as [k v].
+  destruct (key =? k) eqn: eqkey.
+    + apply eqb_eq in eqkey. rewrite -> eqkey. intro Hvalue.
+      unfold domain. unfold In. left. reflexivity.
+    + fold @lookup. (* The @ is needed because of the implicit parameter, otherwise
+                       it cannot infer the type A *)
+      intros Hlookuptail.
+      unfold domain.
+      unfold In.
+      right.
+      fold @domain. 
+      apply IHtail in Hlookuptail.
+      assumption.
+Qed.
+
+
+
+Lemma in_domain_then_lookup: forall {A: Type} (m: map A) (key: string),
+In key (domain m) -> exists (value:A), lookup m key = Some value.
+Proof.
+intros A m key.
+induction m as [ | pair tail].
+- simpl. intro Hfalse. contradiction.
+- destruct (pair) as [k v]. unfold domain.
+  destruct (key =? k) eqn: eqkey.
+  + apply eqb_eq in eqkey. rewrite -> eqkey. intro Hdespl. 
+    exists v. unfold lookup.
+    rewrite -> eqb_refl. reflexivity.
+  + fold @domain. intro Hdespl.
+    destruct Hdespl as [Hkeyfalse|Hintail].
+    * rewrite eqb_neq in eqkey. rewrite Hkeyfalse in eqkey. contradiction.
+    * unfold In in IHtail.
+      apply IHtail in Hintail.
+      unfold lookup.
+      rewrite -> eqkey.
+      fold @lookup.
+      assumption.
+Qed.
+
+
+
+Lemma not_in_domain_then_lookup_none: forall {A: Type} (m: map A) (key: string),
+~In key (domain m) -> lookup m key = None.
+Proof.
+intros A m key.
+induction m as [ | pair tail].
+- simpl. intro Hfalse. reflexivity.
+- destruct (pair) as [k v]. unfold domain.
+  destruct (key =? k) eqn: eqkey.
+  + rewrite -> in_str_equiv_true. 
+    unfold In_list_str_eval.
+    rewrite eqb_sym.
+    rewrite -> eqkey.
+    simpl. 
+    intro Hfalse. contradiction.
+  + simpl. fold @domain. intro Hdespl.
+    pose proof (Decidable.not_or (k = key) (In key (domain tail)) Hdespl) as Hindomain.
+    destruct Hindomain as [Hkkey Hdomaintail].
+    rewrite eqb_sym.
+    rewrite <- eqb_neq in Hkkey.
+    rewrite -> Hkkey.
+    apply IHtail in Hdomaintail.
+    assumption.
+Qed.
+
