README.md
@@ -4,8 +4,14 @@
  
 A fully automated and formally verified tool to verify the semantic equivalence of two loop-free fragments of EVM code.
 
+## Compilation
+
+    $ coq_makefile -f _CoqProject -o Makefile
+    $ make
+
 ## License
 
 The library `lib/evmModel.v`, obtained from https://github.com/ivan71kmayshan27/coq-evm, is licensed under the [GNU Lesser General Public License v3.0](https://www.gnu.org/licenses/lgpl-3.0.html).
 
 The rest of the code is licensed under the [GNU General Public License 3.0](https://www.gnu.org/licenses/gpl-3.0.html), also included in our repository in the `COPYING` file.
+
